Prove correctness of a version of memcpy external to the memory.

new_memory.v
@@ -98,31 +98,30 @@ Section memory_operations.
     ∃ w, MMap m !! x = Some (Obj w).
 
   Global Instance mem_empty: Empty (mem Ti) := Mem ∅.
-
-  Global Instance mem_lookup_mval: Lookup (index * ref) (mval Ti) (mem Ti) :=
-    λ xr m,
-    o ← MMap m !! fst xr;
-    w ← maybe_Obj o;
-    w !! snd xr.
   Global Instance mem_lookup: Lookup (addr Ti) (val Ti) (mem Ti) := λ a m,
     o ← MMap m !! addr_index a;
     w ← maybe_Obj o;
     w' ← w !! addr_ref a;
-    guard (addr_offset a < addr_size a);
+    guard (addr_byte a < addr_byte_size a);
     guard (type_of a ≠ void);
     if decide (addr_is_obj a) then Some (mval_to_val w')
-    else w' !! addr_byte a.
+    else w' !! addr_ref_byte a.
 
   Definition mem_force (a : addr Ti) (m : mem Ti) : mem Ti :=
     match m with
     | Mem m => Mem $ alter (obj_map (alter id (addr_ref a))) (addr_index a) m
     end.
   Global Instance mem_insert: Insert (addr Ti) (val Ti) (mem Ti) := λ a v m,
-    let f (w : mval Ti) : mval Ti :=
-      if decide (addr_is_obj a) then mval_of_val v
-      else <[addr_byte a:=v]>w
+    let f w :=
+      if decide (addr_is_obj a) then mval_of_val v else <[addr_ref_byte a:=v]>w
     in match m with
     | Mem m => Mem $ alter (obj_map (alter f (addr_ref a))) (addr_index a) m
+    end.
+  Fixpoint mem_insert_array (a : addr Ti) (vs : list (val Ti))
+      (m : mem Ti) : mem Ti :=
+    match vs with
+    | [] => m
+    | v :: vs => <[a:=v]>(mem_insert_array (addr_plus 1 a) vs m)
     end.
 
   Definition is_free (x : index) (m : mem Ti) := MMap m !! x = None.
@@ -263,9 +262,9 @@ Lemma mem_lookup_Some m a v :
     type_of_index m (addr_index a) = Some τ ∧
     m ⊢ w : τ ∧ addr_ref a @ τ ↣ τ' ∧
     w !! addr_ref a = Some w' ∧ m ⊢ w' : τ' ∧
-    addr_offset a < addr_size a ∧ type_of a ≠ void ∧
+    addr_byte a < addr_byte_size a ∧ type_of a ≠ void ∧
     (addr_is_obj a → v = mval_to_val w') ∧
-    (¬addr_is_obj a → w' !! addr_byte a = Some v).
+    (¬addr_is_obj a → w' !! addr_ref_byte a = Some v).
 Proof.
   intros Hm Hav. unfold lookup, mem_lookup in Hav.
   destruct (MMap m !! addr_index a) as [o|] eqn:Ho; simplify_equality'.
@@ -342,14 +341,14 @@ Lemma type_of_index_force m a τ y σ :
 Proof.
   intros Hm Ha Hy. destruct m as [m].
   unfold type_of_index, mem_type_of_index, mem_force in *; simpl in *.
-  destruct (decide (addr_index a = y)); simplify_option_equality.
-  * rewrite lookup_alter.
-    destruct (m !! addr_index a) as [[|w]|] eqn:?; simplify_equality'; auto.
-    destruct (addr_typed_ref_alt (Mem m) a τ) as (?&?&?); auto.
-    destruct (mem_lookup_raw_Obj (Mem m) (addr_index a) w) as (τ'&?&?&_); auto.
-    simplify_type_equality; simplify_option_equality.
-    f_equal. eapply type_of_correct with (Mem m), mval_alter_typed; eauto.
-  * rewrite lookup_alter_ne by done. by simplify_option_equality.
+  destruct (decide (addr_index a = y)); simplify_option_equality;
+    [|by rewrite lookup_alter_ne; simplify_option_equality].
+  rewrite lookup_alter.
+  destruct (m !! addr_index a) as [[|w]|] eqn:?; simplify_equality'; auto.
+  destruct (addr_typed_ref_base (Mem m) a τ) as (?&?&?); auto.
+  destruct (mem_lookup_raw_Obj (Mem m) (addr_index a) w) as (τ'&?&?&_); auto.
+  simplify_type_equality; simplify_option_equality.
+  f_equal. eapply type_of_correct with (Mem m), mval_alter_typed; eauto.
 Qed.
 Lemma addr_typed_force m a τ a' σ :
   ⊢ valid m → m ⊢ a : τ → m ⊢ a' : σ → mem_force a m ⊢ a' : σ.
@@ -366,79 +365,120 @@ Proof. eauto using mtyped_weaken_mem, type_of_index_force. Qed.
 Lemma obj_typed_force m a τ o σ :
   ⊢ valid m → m ⊢ a : τ → m ⊢ o : σ → mem_force a m ⊢ o : σ.
 Proof. eauto using obj_typed_weaken_mem, type_of_index_force. Qed.
-
-Lemma type_of_index_insert m a v τ y σ :
-  ⊢ valid m → m ⊢ a : τ → m ⊢ v : τ →
-  type_of_index m y = Some σ → type_of_index (<[a:=v]>m) y = Some σ.
-Proof.
-  intros Hm Haτ Hvτ Hy. destruct m as [m]; unfold type_of_index,
-    mem_type_of_index, insert, mem_insert in *; simpl in *.
-  destruct (decide (addr_index a = y)); simplify_equality.
-  * rewrite lookup_alter.
-    destruct (addr_typed_ref_alt (Mem m) a τ) as (?&?&?); auto.
-    unfold type_of_index, mem_type_of_index in *.
-    destruct (m !! addr_index a) as [[?|w]|] eqn:Hw; simplify_equality'; auto.
-    destruct (Hm (addr_index a) (Obj w)) as (τ'&Hwτ&?); auto.
-    inversion Hwτ; simplify_option_equality; simplify_type_equality.
-    f_equal; eapply type_of_correct with (Mem m), mval_alter_typed; eauto.
-    intros ??. repeat case_decide; simplify_type_equality.
-    + erewrite addr_is_obj_type_base by eauto. eauto using mval_of_val_typed.
-    + eapply mval_insert_byte_typed; auto.
-      by rewrite <-(addr_not_is_obj_type (Mem m) a τ)
-        by eauto using vtyped_not_void.
-  * by rewrite lookup_alter_ne.
-Qed.
-Lemma addr_typed_insert m a v τ a' σ :
-  ⊢ valid m → m ⊢ a : τ → m ⊢ v : τ → m ⊢ a' : σ → <[a:=v]>m ⊢ a' : σ.
-Proof. eauto using addr_typed_weaken_mem, type_of_index_insert. Qed.
-Lemma ptr_typed_insert m a v τ p σ :
-  ⊢ valid m → m ⊢ a : τ → m ⊢ v : τ → m ⊢ p : σ → <[a:=v]>m ⊢ p : σ.
-Proof. eauto using ptr_typed_weaken_mem, type_of_index_insert. Qed.
-Lemma vtyped_insert m a v τ v' σ :
-  ⊢ valid m → m ⊢ a : τ → m ⊢ v : τ → m ⊢ v' : σ → <[a:=v]>m ⊢ v' : σ.
-Proof. eauto using vtyped_weaken_mem, type_of_index_insert. Qed.
-Lemma mtyped_insert m a v τ w σ :
-  ⊢ valid m → m ⊢ a : τ → m ⊢ v : τ → m ⊢ w : σ → <[a:=v]>m ⊢ w : σ.
-Proof. eauto using mtyped_weaken_mem, type_of_index_insert. Qed.
-Lemma obj_typed_insert m a v τ o σ :
-  ⊢ valid m → m ⊢ a : τ → m ⊢ v : τ → m ⊢ o : σ → <[a:=v]>m ⊢ o : σ.
-Proof. eauto using obj_typed_weaken_mem, type_of_index_insert. Qed.
-
-Lemma mem_force_typed m a σ : ⊢ valid m → m ⊢ a : σ → ⊢ valid (mem_force a m).
+Lemma mem_force_valid m a σ : ⊢ valid m → m ⊢ a : σ → ⊢ valid (mem_force a m).
 Proof.
   destruct m as [m]; intros Hm Ha x o Hx; simpl in *.
   rewrite lookup_alter_Some in Hx.
   destruct Hx as [(<-&o'&?&->)|[??]]; simplify_option_equality.
-  * destruct (addr_typed_ref_alt (Mem m) a σ) as (τ&?&?); auto.
+  * destruct (addr_typed_ref_base (Mem m) a σ) as (τ&?&?); auto.
     destruct (mem_lookup_raw (Mem m) (addr_index a) o') as (?&?&?&?); auto.
     simplify_option_equality; simplify_type_equality.
     exists τ; split; auto. apply obj_map_typed.
-    + eauto using mval_alter_typed.
+    + intros. eapply mval_alter_typed; eauto.
     + eapply (obj_typed_force (Mem m)); eauto.
   * destruct (mem_lookup_raw (Mem m) x o) as (τ&?&_&?);
       simplify_type_equality; auto.
     exists τ; split; auto. eapply (obj_typed_force (Mem m)); eauto.
 Qed.
-Lemma mem_insert_typed m a v σ :
-  ⊢ valid m → m ⊢ a : σ → m ⊢ v : σ → ⊢ valid (<[a:=v]>m).
+
+Lemma type_of_index_insert m a j v τ y σ :
+  ⊢ valid m → m ⊢ a : τ → m ⊢ v : τ →
+  type_of_index m y = Some σ →
+  type_of_index (<[addr_plus j a:=v]>m) y = Some σ.
+Proof.
+  intros Hm Haτ Hvτ Hy. destruct m as [m]; unfold type_of_index,
+    mem_type_of_index, insert, mem_insert in *; simpl in *.
+  rewrite addr_index_plus.
+  destruct (decide (addr_index a = y)); simplify_equality;
+    [rewrite lookup_alter | by rewrite lookup_alter_ne].
+  destruct (addr_typed_ref_base (Mem m) a τ) as (?&Hx&Hr); auto.
+  unfold type_of_index, mem_type_of_index in Hx.
+  destruct (m !! addr_index a) as [[?|w]|] eqn:Hw; simplify_equality'; auto.
+  destruct (Hm (addr_index a) (Obj w)) as (τ'&Hwτ&_); auto.
+  inversion Hwτ; simplify_option_equality; simplify_type_equality.
+  f_equal; eapply type_of_correct with (Mem m).
+  eapply mval_alter_typed; rewrite ?addr_ref_base_plus; eauto.
+  intros ??. case_decide as Hobj; rewrite addr_is_obj_plus in Hobj;
+    simplify_type_equality.
+  * erewrite addr_is_obj_type_base by eauto.
+    eauto using mval_of_val_typed.
+  * eapply mval_insert_byte_typed; auto.
+    by rewrite <-(addr_not_is_obj_type (Mem m) a τ) by
+      (rewrite ?addr_is_obj_plus; eauto using vtyped_not_void).
+Qed.
+Lemma addr_typed_insert m a j v τ a' σ :
+  ⊢ valid m → m ⊢ a : τ → m ⊢ v : τ →
+  m ⊢ a' : σ → <[addr_plus j a:=v]>m ⊢ a' : σ.
+Proof. eauto using addr_typed_weaken_mem, type_of_index_insert. Qed.
+Lemma ptr_typed_insert m a j v τ p σ :
+  ⊢ valid m → m ⊢ a : τ → m ⊢ v : τ →
+  m ⊢ p : σ → <[addr_plus j a:=v]>m ⊢ p : σ.
+Proof. eauto using ptr_typed_weaken_mem, type_of_index_insert. Qed.
+Lemma vtyped_insert m a j v τ v' σ :
+  ⊢ valid m → m ⊢ a : τ → m ⊢ v : τ →
+  m ⊢ v' : σ → <[addr_plus j a:=v]>m ⊢ v' : σ.
+Proof. eauto using vtyped_weaken_mem, type_of_index_insert. Qed.
+Lemma mtyped_insert m a j v τ w σ :
+  ⊢ valid m → m ⊢ a : τ → m ⊢ v : τ →
+  m ⊢ w : σ → <[addr_plus j a:=v]>m ⊢ w : σ.
+Proof. eauto using mtyped_weaken_mem, type_of_index_insert. Qed.
+Lemma obj_typed_insert m a j v τ o σ :
+  ⊢ valid m → m ⊢ a : τ → m ⊢ v : τ →
+  m ⊢ o : σ → <[addr_plus j a:=v]>m ⊢ o : σ.
+Proof. eauto using obj_typed_weaken_mem, type_of_index_insert. Qed.
+Lemma mem_insert_valid m a j v σ :
+  ⊢ valid m → m ⊢ a : σ → m ⊢ v : σ → ⊢ valid (<[addr_plus j a:=v]>m).
 Proof.
   destruct m as [m]; intros Hm Ha Hv x o Hx; simpl in *.
-  rewrite lookup_alter_Some in Hx.
+  rewrite !addr_index_plus, lookup_alter_Some in Hx.
   destruct Hx as [(<-&o'&?&->)|[??]]; simplify_option_equality.
-  * destruct (addr_typed_ref_alt (Mem m) a σ) as (τ&?&?); auto.
+  * destruct (addr_typed_ref_base (Mem m) a σ) as (τ&?&?); auto.
     destruct (mem_lookup_raw (Mem m) (addr_index a) o') as (?&?&?&?); auto.
     simplify_option_equality; simplify_type_equality.
     exists τ; split; auto. apply obj_map_typed; eauto using obj_typed_insert.
-    intros w Hw. eapply mval_alter_typed; eauto.
-    intros w' Hw'. repeat case_decide; simplify_type_equality.
-    + erewrite addr_is_obj_type_base by eauto. apply mval_of_val_typed.
+    intros w Hw. eapply mval_alter_typed; rewrite ?addr_ref_base_plus; eauto.
+    intros w' Hw'. case_decide as Hobj; simplify_type_equality.
+    + rewrite addr_is_obj_plus in Hobj.
+      erewrite addr_is_obj_type_base by eauto. apply mval_of_val_typed.
       eauto using vtyped_insert.
     + eapply mval_insert_byte_typed; auto.
+      rewrite addr_is_obj_plus in Hobj.
       rewrite <-(addr_not_is_obj_type (Mem m) a σ)
          by eauto using vtyped_not_void; eauto using vtyped_insert.
   * destruct (mem_lookup_raw (Mem m) x o) as (τ&?&_&?);
       simplify_type_equality; eauto using obj_typed_insert.
 Qed.
+
+Lemma mem_insert_array_app m a vs1 vs2 :
+  mem_insert_array a (vs1 ++ vs2) m = mem_insert_array a vs1 $
+    mem_insert_array (addr_plus (length vs1) a) vs2 m.
+Proof.
+  revert a. induction vs1 as [|v1 vs1 IH]; intros a; simpl.
+  { by rewrite addr_plus_0. }
+  rewrite Zpos_P_of_succ_nat, IH.
+  by rewrite addr_plus_plus, Z.add_1_r by auto with zpos.
+Qed.
+
+(* todo, generalize for (j : Z) *)
+Lemma type_of_index_insert_array_help m a (j : nat) vs τ y :
+  ⊢ valid m → m ⊢ a : τ → m ⊢* vs : τ →
+  (∀ σ, type_of_index m y = Some σ →
+    type_of_index (mem_insert_array (addr_plus j a) vs m) y = Some σ) ∧
+  ⊢ valid (mem_insert_array (addr_plus j a) vs m) ∧
+  (∀ a' σ, m ⊢ a' : σ → mem_insert_array (addr_plus j a) vs m ⊢ a' : σ) ∧
+  (∀ v σ, m ⊢ v : σ → mem_insert_array (addr_plus j a) vs m ⊢ v : σ).
+Proof.
+  intros Hm Haτ Hvs. revert j.
+  induction Hvs as [|v vs Hv Hvs IH]; simpl; auto.
+  intros j; destruct (IH (1 + j)) as (?&?&?&?).
+  rewrite !(addr_plus_plus_nat _ 1). naive_solver eauto using
+    type_of_index_insert, mem_insert_valid, addr_typed_insert, vtyped_insert.
+Qed.
+Lemma type_of_index_insert_array m a (j : nat) vs τ y σ :
+  ⊢ valid m → m ⊢ a : τ → m ⊢* vs : τ →
+  type_of_index m y = Some σ →
+  type_of_index (mem_insert_array (addr_plus j a) vs m) y = Some σ.
+Proof. intros. eapply type_of_index_insert_array_help; eauto. Qed.
 
 Lemma mem_lookup_insert m a v σ :
   ⊢ valid m → m ⊢ a : σ → is_Some (m !! a) → addr_is_obj a →
@@ -498,11 +538,11 @@ Proof.
     feed pose proof (addr_not_is_obj_type (Mem m) a2 τ2);
       eauto using vtyped_not_void; subst.
     f_equal. rewrite <-!(mval_alter_freeze _ (addr_ref a1)),
-      <-!(mval_alter_freeze _ (addr_ref a2)), <-!Ha, <-!mval_alter_compose.
-    destruct (addr_typed_ref_alt (Mem m) a1 uchar) as (σ&?&?); auto.
+      <-!(mval_alter_freeze _ (addr_ref a2)), <-!Ha.
+    rewrite !mval_alter_freeze, <-!mval_alter_compose.
+    destruct (addr_typed_ref_base (Mem m) a1 uchar) as (σ&?&?); auto.
     simplify_option_equality.
-    apply (mval_alter_ext_typed (Mem m) _ _ _ τ 0 _ (addr_type_base a1)); auto.
-    { rewrite ref_set_offset_freeze. by apply ref_typed_freeze. }
+    apply (mval_alter_ext_typed (Mem m) _ _ _ τ _ _ (addr_type_base a1)); auto.
     intros w' Hw'; simpl.
     by repeat case_decide; eauto using mval_insert_byte_commute.
 Qed.
@@ -538,20 +578,23 @@ Lemma mem_aliasing_help m a1 a2 σ1 σ2 :
   (* 1.) *) (∀ j1 j2, addr_plus j1 a1 ⊥ addr_plus j2 a2) ∨
   (* 2.) *) σ1 ⊆ σ2 ∨
   (* 3.) *) σ2 ⊆ σ1 ∨
-  (* 4.) *) ∀ f,
-    mem_alter f a2 !! a1 = None ∧
-    mem_alter f a1 !! a2 = None.
+  (* 4.) *) ∀ f j1 j2,
+    mem_alter f (addr_plus j2 a2) !! addr_plus j1 a1 = None ∧
+    mem_alter f (addr_plus j1 a1) !! addr_plus j2 a2 = None.
 Proof.
   intros. destruct (addr_disjoint_cases m a1 a2 σ1 σ2)
     as [Ha12|[?|[?|(Hidx&s&r1'&i1&r2'&i2&r'&Ha1&Ha2&?)]]]; auto.
-  do 3 right. intros f. unfold mem_alter, lookup, mem_lookup, mem_force.
-  destruct m as [m]; simpl. rewrite <-!Hidx, !lookup_alter, Ha1, Ha2.
+  do 3 right. intros f j1 j2. unfold mem_alter, lookup, mem_lookup, mem_force.
+  destruct m as [m]; simpl.
+  rewrite !addr_index_plus, <-!Hidx, !lookup_alter.
   destruct (m !! addr_index a1) as [[|w]|] eqn:Hw; simpl; auto.
   destruct (mem_lookup_raw_Obj (Mem m) (addr_index a1) w) as (τ&?&?&_); auto.
-  destruct (addr_typed_ref_alt (Mem m) a1 σ1) as (τ'&Hidx1&Hr1); auto.
-  destruct (addr_typed_ref_alt (Mem m) a2 σ2) as (τ''&Hidx2&Hr2); auto.
-  rewrite <-Hidx in Hidx2. rewrite Ha1 in Hr1. rewrite Ha2 in Hr2.
-  simplify_option_equality. by erewrite !mval_lookup_non_aliasing by eauto.
+  destruct (addr_typed_ref_base (Mem m) a1 σ1) as (τ'&Hidx1&Hr1); auto.
+  destruct (addr_typed_ref_base (Mem m) a2 σ2) as (τ''&Hidx2&Hr2); auto.
+  rewrite <-Hidx in Hidx2; rewrite Ha1 in Hr1; rewrite Ha2 in Hr2.
+  unfold addr_ref;
+    rewrite !addr_ref_base_plus, Ha1, Ha2; simplify_option_equality.
+  by erewrite !mval_lookup_non_aliasing by eauto.
 Qed.
 Lemma mem_aliasing m a1 a2 σ1 σ2 :
   ⊢ valid m → m ⊢ a1 : σ1 → m ⊢ a2 : σ2 →
@@ -559,18 +602,18 @@ Lemma mem_aliasing m a1 a2 σ1 σ2 :
   (* 1.) *) (∀ j1 j2, addr_plus j1 a1 ⊥ addr_plus j2 a2) ∨
   (* 2.) *) σ1 ⊆ σ2 ∨
   (* 3.) *) σ2 ⊆ σ1 ∨
-  (* 4.) *)
-    (∀ v1, <[a1:=v1]>m !! a2 = None) ∧
-    mem_force a1 m !! a2 = None ∧
-    (∀ v2, <[a2:=v2]>m !! a1 = None) ∧
-    mem_force a2 m !! a1 = None.
+  (* 4.) *) ∀ j1 j2,
+    (∀ v1, <[addr_plus j1 a1:=v1]>m !! addr_plus j2 a2 = None) ∧
+    mem_force (addr_plus j1 a1) m !! addr_plus j2 a2 = None ∧
+    (∀ v2, <[addr_plus j2 a2:=v2]>m !! addr_plus j1 a1 = None) ∧
+    mem_force (addr_plus j2 a2) m !! addr_plus j1 a1 = None.
 Proof.
   intros. destruct (mem_aliasing_help m a1 a2 σ1 σ2) as [?|[?|[?|Hf]]]; auto.
-  do 3 right. destruct m as [m]. split_ands.
-  * intros. unfold insert, mem_insert; simpl. by rewrite (proj2 (Hf _)).
-  * intros. unfold mem_force; simpl. by rewrite (proj2 (Hf _)).
-  * intros. unfold insert, mem_insert; simpl. by rewrite (proj1 (Hf _)).
-  * intros. unfold mem_force; simpl. by rewrite (proj1 (Hf _)).
+  do 3 right. destruct m as [m]. intros j1 j2; split_ands.
+  * intros. unfold insert, mem_insert; simpl. by rewrite (proj2 (Hf _ _ _)).
+  * intros. unfold mem_force; simpl. by rewrite (proj2 (Hf _ _ _)).
+  * intros. unfold insert, mem_insert; simpl. by rewrite (proj1 (Hf _ _ _)).
+  * intros. unfold mem_force; simpl. by rewrite (proj1 (Hf _ _ _)).
 Qed.
 
 Lemma type_of_index_mem_le m1 m2 y σ :
@@ -611,7 +654,7 @@ Proof.
   destruct (decide (addr_is_obj a)).
   { exists (mval_to_val w4). rewrite Hobj by done. split; auto.
     eapply mval_to_val_le; eauto using mtyped_mem_le. }
-  destruct (mval_lookup_byte_le m2 w3 w4 τ3 (addr_byte a) v1)
+  destruct (mval_lookup_byte_le m2 w3 w4 τ3 (addr_ref_byte a) v1)
     as (v2&?&?); eauto using mtyped_mem_le.
 Qed.
 Lemma mem_lookup_ge m1 m2 a v2 :
@@ -629,34 +672,36 @@ Proof.
   right. destruct (decide (addr_is_obj a)).
   { exists (mval_to_val w3). rewrite Hobj by done. split; auto.
     eapply mval_to_val_le; eauto using mtyped_le. }
-  destruct (mval_lookup_byte_ge m2 w3 w4 τ4 (addr_byte a) v2)
+  destruct (mval_lookup_byte_ge m2 w3 w4 τ4 (addr_ref_byte a) v2)
     as (v1&?&?); eauto using mtyped_le.
 Qed.
-Lemma mem_insert_le m1 m2 a σ v1 v2 :
+Lemma mem_insert_le m1 m2 a j σ v1 v2 :
   ⊢ valid m2 → m1 ⊆ m2 → m2 ⊢ a : σ → m2 ⊢ v1 : σ →
-  v1 ⊑@{m2} v2 → <[a:=v1]>m1 ⊆ <[a:=v2]>m2.
+  v1 ⊑@{m2} v2 → <[addr_plus j a:=v1]>m1 ⊆ <[addr_plus j a:=v2]>m2.
 Proof.
   destruct m1 as [m1], m2 as [m2]. unfold insert, mem_insert.
-  intros Hm Hm12 Ha Hv1 Hv12 x o1; simpl. rewrite lookup_alter_Some.
-  intros [(<-&o1'&?&->)|[??]].
+  intros Hm Hm12 Ha Hv1 Hv12 x o1; simpl.
+  rewrite addr_index_plus, lookup_alter_Some. intros [(<-&o1'&?&->)|[??]].
   * destruct (Hm12 (addr_index a) o1') as (o2&Ho2&Ho12); simpl in *; auto.
     rewrite lookup_alter, Ho2; simpl. eexists; split; auto.
     apply obj_le_weaken_mem with (Mem m2); auto.
-    { intros ??.
+    { intros ??. rewrite <-(addr_index_plus a j).
       eapply (type_of_index_insert (Mem m2)); eauto using vtyped_ge. }
     inversion Ho12; subst; clear Ho12; constructor.
-    destruct (addr_typed_ref_alt (Mem m2) a σ) as (τ&?&?); auto.
+    destruct (addr_typed_ref_base (Mem m2) a σ) as (τ&?&?); auto.
     destruct (mem_lookup_raw_Obj (Mem m2) (addr_index a) w2)
       as (?&?&?&_); auto; simplify_option_equality.
-    eapply mval_alter_le; eauto using mtyped_le.
-    intros w3 s4 ??. repeat case_decide; eauto using mval_of_val_le.
+    eapply mval_alter_le; rewrite ?addr_ref_base_plus; eauto using mtyped_le.
+    intros w3 s4 ??. case_decide as Hobj; eauto using mval_of_val_le.
+    rewrite addr_is_obj_plus in Hobj.
     eapply mval_insert_byte_le; eauto.
     by rewrite <-(addr_not_is_obj_type (Mem m2) a σ)
       by eauto using vtyped_not_void.
   * destruct (Hm12 x o1) as (o2&?&?); auto. exists o2.
     rewrite !lookup_alter_ne by done. split; auto.
     apply obj_le_weaken_mem with (Mem m2); auto.
-    intros ??. eapply (type_of_index_insert (Mem m2)); eauto using vtyped_ge.
+    intros ??. rewrite <-(addr_index_plus a j).
+    eapply (type_of_index_insert (Mem m2)); eauto using vtyped_ge.
 Qed.
 Lemma mem_force_le m1 m2 a σ :
   ⊢ valid m2 → m1 ⊆ m2 → m2 ⊢ a : σ → mem_force a m1 ⊆ mem_force a m2.
@@ -669,7 +714,7 @@ Proof.
     apply obj_le_weaken_mem with (Mem m2); auto.
     { intros ??. eapply (type_of_index_force (Mem m2)); eauto. }
     inversion Ho12; subst; clear Ho12; constructor.
-    destruct (addr_typed_ref_alt (Mem m2) a σ) as (τ&?&?); auto.
+    destruct (addr_typed_ref_base (Mem m2) a σ) as (τ&?&?); auto.
     destruct (mem_lookup_raw_Obj (Mem m2) (addr_index a) w2)
       as (?&?&?&_); auto; simplify_option_equality.
     eapply mval_alter_le; eauto using mtyped_le.
@@ -702,5 +747,174 @@ Proof.
     rewrite lookup_alter_ne by done. split; auto.
     apply obj_le_weaken_mem with (Mem m2); auto.
     intros ??. apply (type_of_index_delete (Mem m2)).
+Qed.
+
+Lemma mem_lookup_value_bytes m a v σ :
+  ⊢ valid m → m ⊢ a : σ → m !! a = Some v → ∃ cs,
+  (* a.) *) length cs = size_of σ ∧
+  (* b.) *) m ⊢* cs : uchar ∧
+  (* c.) *) (∀ j : nat,
+    j < size_of σ → m !! addr_plus j (addr_cast uchar a) = cs !! j) ∧
+  (* d.) *) val_to_bits v ⊑@{m}* mjoin (val_to_bits <$> cs).
+Proof.
+  intros Hm Ha Hav. pose proof (mem_lookup_Some _ _ _ Hm Hav) as Hav'.
+  destruct Hav' as (w&τ&w'&τ'&Hma&?&?&?&Hwa&Hw'&?&?&Hobj&Hbyte).
+  destruct (decide (addr_is_obj a)) as [Ha1|Ha1].
+  { specialize (Hobj Ha1); subst.
+    feed pose proof (addr_typed_ref_type_base_inv m a σ τ τ'); auto; subst.
+    erewrite addr_is_obj_type_base in Hw' by eauto; simplify_type_equality'.
+    exists (val_of_bits uchar <$>
+      reshape (replicate (size_of σ) char_bits) (mval_to_bits w')); split_ands.
+    * by rewrite fmap_length, reshape_length, replicate_length.
+    * eapply Forall_fmap, Forall_impl;
+        [eapply Forall_reshape, mval_to_bits_valid; eauto |].
+      eauto using val_of_bits_typed, TBase_valid, TInt_valid.
+    * intros j Hj. unfold lookup at 1, mem_lookup.
+      rewrite addr_index_plus, addr_index_cast, Hma; simpl.
+      erewrite list_lookup_fmap, <-mval_lookup_reshape by eauto.
+      erewrite addr_ref_plus_char_cast, Hwa by eauto; simpl.
+      rewrite option_guard_True by (rewrite addr_byte_size_plus,
+        addr_byte_size_cast; eauto using addr_byte_lt_size_char_cast).
+      rewrite option_guard_True by (by rewrite addr_type_plus, addr_type_cast).
+      case_decide as Hobj.
+      + erewrite addr_is_obj_plus, addr_is_obj_cast,
+          addr_is_obj_type_base in Hobj by eauto; simplify_equality.
+        replace j with 0 by (rewrite size_of_int, int_size_char in Hj; lia).
+        by erewrite mval_lookup_byte_char by eauto.
+      + by erewrite addr_ref_byte_plus_char_cast by eauto.
+    * assert (Forall (λ bs, val_to_bits (val_of_bits uchar bs) = bs)
+        (reshape (replicate (size_of σ) char_bits) (mval_to_bits w'))).
+      { generalize (mval_to_bits_length _ _ _ Hw'); unfold bit_size_of.
+        rewrite <-(int_bits_char Unsigned), <-bit_size_of_int.
+        generalize (mval_to_bits w').
+        induction (size_of σ) as [|n IH]; intros bs; simpl; constructor; auto.
+        + rewrite val_of_bits_base; unfold val_to_bits; simpl.
+          by rewrite base_val_to_of_bits_char by (rewrite take_length_le; lia).
+        + apply IH. rewrite drop_length. lia. }
+      erewrite <-list_fmap_compose, (proj1 (Forall_fmap_ext _ id _)) by done.
+      rewrite list_fmap_id, join_reshape by
+        (by erewrite sum_list_replicate, mval_to_bits_length by eauto).
+      eapply mval_to_bits_le, mval_of_to_val; eauto. }
+  simplify_type_equality.
+  feed pose proof (addr_not_is_obj_type m a σ); auto; subst.
+  rewrite size_of_int, int_size_char. exists [v]; split_ands; auto.
+  * apply Forall_singleton. eauto using mval_lookup_byte_typed.
+  * intros [|?] ?; auto with lia; simpl.
+    by erewrite addr_plus_0, addr_cast_self by eauto.
+  * by simpl; rewrite (right_id_L [] (++)).
+Qed.
+
+Lemma mem_lookup_insert_raw m a v x :
+  addr_index a = x →
+  let f w :=
+   if decide (addr_is_obj a) then mval_of_val v else <[addr_ref_byte a:=v]> w in
+  MMap (<[a:=v]>m) !! x = obj_map (alter f (addr_ref a)) <$> MMap m !! x.
+Proof. intros <-. destruct m as [m]; simpl. by rewrite lookup_alter. Qed.
+Lemma mem_lookup_insert_ne_raw m a v x  :
+  addr_index a ≠ x → MMap (<[a:=v]>m) !! x = MMap m !! x.
+Proof. intros. destruct m as [m]; simpl. by rewrite lookup_alter_ne. Qed.
+
+Lemma mem_lookup_insert_array_raw m a σ (j : nat) cs :
+  ⊢ valid m → m ⊢ a : σ → addr_is_obj a →
+  m ⊢* cs : uchar → length cs + j = size_of σ → 0 < length cs →
+  MMap (mem_insert_array (addr_plus j (addr_cast uchar a)) cs m)
+    !! addr_index a = obj_map (alter (mval_insert_bytes j cs) (addr_ref a))
+                      <$> MMap m !! addr_index a.
+Proof.
+  intros Hm Haσ Hobj Hcs; revert j.
+  destruct (decide (addr_is_obj (addr_cast uchar a))) as [Hobj'|?].
+  { intros j Hj Hlen. rewrite addr_is_obj_cast in Hobj'.
+    erewrite addr_is_obj_type_base in Hobj' by eauto. subst.
+    rewrite size_of_int, int_size_char in Hj.
+    destruct cs as [|c []]; simplify_equality'; auto with lia.
+    rewrite Forall_singleton in Hcs.
+    rewrite mem_lookup_insert_raw by (by destruct a).
+    destruct (MMap m !! _) as [[|w]|] eqn:Hw; simpl; do 2 f_equal.
+    destruct (mem_lookup_raw_Obj m (addr_index a) w) as (τ&?&?&_); auto.
+    destruct (addr_typed_ref_base m a uchar) as (τ'&?&?); auto.
+    simplify_option_equality. rewrite addr_plus_0, addr_ref_cast.
+    eapply mval_alter_ext_typed; eauto. intros w' Hw'. case_decide as Hobj'.
+    { rewrite addr_is_obj_cast in Hobj'; rewrite <-Hobj' in Hw'.
+      by erewrite mval_insert_byte_char by eauto. }
+    by erewrite addr_ref_byte_cast, addr_is_obj_ref_byte by eauto. }
+  induction Hcs as [|c1 cs Hc1 Hcs IH]; simpl; intros j Hj Hlen; auto with lia.
+  destruct (nil_or_length_pos cs); simplify_equality'.
+  { rewrite mem_lookup_insert_raw by (by destruct a).
+    destruct (MMap m !! _) as [[|w]|]; simpl; do 2 f_equal.
+    erewrite addr_ref_plus_char_cast by eauto with lia.
+    eapply mval_alter_ext; intros w'. case_decide as Hobj'.
+    * by rewrite addr_is_obj_plus in Hobj'.
+    * by erewrite addr_ref_byte_plus_char_cast by eauto with lia. }
+  rewrite (addr_plus_plus_nat _ 1 j).
+  rewrite mem_lookup_insert_raw by (by destruct a); rewrite IH by lia.
+  destruct (MMap m !! _) as [[|w]|]; simpl; do 2 f_equal.
+  erewrite addr_ref_plus_char_cast by eauto with lia.
+  rewrite <-mval_alter_compose.
+  eapply mval_alter_ext; intros w'. case_decide as Hobj'.
+  * by rewrite addr_is_obj_plus in Hobj'.
+  * simpl. by erewrite addr_ref_byte_plus_char_cast by eauto with lia.
+Qed.
+Lemma mem_lookup_insert_array_ne_raw m a cs x :
+  addr_index a ≠ x → MMap (mem_insert_array a cs m) !! x = MMap m !! x.
+Proof.
+  revert a. induction cs as [|c cs IH]; simpl; intros; auto.
+  by rewrite mem_lookup_insert_ne_raw, IH by (by rewrite ?addr_index_plus).
+Qed.
+
+Lemma mem_insert_value_bytes m a v σ cs :
+  ⊢ valid m → m ⊢ a : σ → addr_strict m a → m ⊢ v : σ →
+  length cs = size_of σ → m ⊢* cs : uchar →
+  val_to_bits v ⊑@{m}* mjoin (val_to_bits <$> cs) →
+  <[a:=v]>m ⊆ mem_insert_array (addr_cast uchar a) cs m.
+Proof.
+  destruct m as [m]; intros Hm Haσ Ha Hvσ Hlen Hcs Hvcs x o; simpl.
+  rewrite lookup_alter_Some. intros [(<-&o'&Hx&->)|[? Hx]].
+  { destruct (mem_lookup_raw (Mem m) (addr_index a) o') as (τ&Ho'&?&_); auto.
+    destruct (addr_typed_ref_base (Mem m) a σ) as (τ'&?&Hr); auto.
+    simplify_option_equality. destruct (decide (addr_is_obj a)).
+    * erewrite addr_is_obj_type_base in Hr by eauto.
+      exists (obj_map (alter (λ _, mval_of_bits σ $
+        mjoin (val_to_bits <$> cs)) (addr_ref a)) o'); split.
+      { rewrite <-(addr_plus_0 (addr_cast _ _)).
+        feed pose proof (size_of_pos σ); eauto using vtyped_type_valid.
+        erewrite (mem_lookup_insert_array_raw _ _ _ 0); eauto with lia; simpl.
+        rewrite Hx. destruct Ho' as [|w τ Hw]; simpl; do 2 f_equal; auto.
+        eapply mval_alter_ext_typed; eauto using mval_insert_bytes_join. }
+      apply obj_le_weaken_mem with (Mem m).
+      { intros ??. rewrite <-(addr_plus_0 (addr_cast uchar a)).
+        eapply (type_of_index_insert_array _ _ 0);
+          eauto using addr_cast_ok_typed, addr_cast_ok_uchar. }
+      destruct Ho' as [|w τ Hw]; constructor.
+      eapply mval_alter_le; eauto; intros w3 w4 ??.
+      transitivity (mval_of_bits σ (val_to_bits v)).
+      { unfold val_to_bits.
+        erewrite mval_of_to_bits by eauto using mval_of_val_typed.
+        eapply munion_reset_above; eauto using mval_of_val_typed. }
+      eapply mval_of_bits_le; eauto using vtyped_type_valid.
+    * feed pose proof (addr_not_is_obj_type (Mem m) a σ);
+        eauto using vtyped_not_void; subst.
+      rewrite size_of_int, int_size_char in Hlen.
+      destruct Hcs as [|c ? Hc []]; simplify_equality'.
+      rewrite (right_id_L [] (++)) in Hvcs.
+      apply (val_of_bits_le _ uchar) in Hvcs;
+        eauto using TBase_valid, TInt_valid, val_to_bits_valid.
+      erewrite !val_of_to_bits in Hvcs by eauto using union_free_base.
+      erewrite !val_frozen_freeze in Hvcs by eauto using val_frozen_int.
+      rewrite addr_index_cast, lookup_alter, Hx.
+      rewrite addr_ref_cast, addr_ref_byte_cast.
+      eexists; split; [done|]. apply obj_le_weaken_mem with (Mem m).
+      { intros ??. rewrite <-(addr_plus_0 (addr_cast uchar a)).
+        eapply (type_of_index_insert _ _ 0);
+          eauto using addr_cast_ok_typed, addr_cast_ok_uchar. }
+      destruct Ho' as [|w τ Hw]; constructor.
+      eapply mval_alter_le; eauto; intros w3 w4 Hw3 ?. case_decide as Hobj.
+      { feed pose proof (addr_byte_range (Mem m) a uchar) as Hbyte; auto.
+        rewrite addr_is_obj_cast in Hobj. rewrite <-Hobj in Hw3, Hbyte.
+        rewrite size_of_int, int_size_char in Hbyte.
+        replace (addr_ref_byte a) with 0 by lia.
+        erewrite mval_insert_byte_char by eauto. eauto using mval_of_val_le. }
+      eauto using mval_insert_byte_le. }
+  exists o. split; auto.
+  by rewrite mem_lookup_insert_array_ne_raw by (by destruct a).
 Qed.
 End memory.
